Splinter/SplinterTree.i.dfy
@@ -9,7 +9,7 @@ include "AllocationTable.i.dfy"
 include "AllocationTableMachine.i.dfy"
 include "MsgHistory.i.dfy"
 include "../Spec/Message.s.dfy"
-include "../Spec/Interp.s.dfy"
+include "../Spec/StampedMap.s.dfy"
 include "BranchTree.i.dfy"
 include "BranchTreeInterp.i.dfy"
 include "MsgSeq.i.dfy"
@@ -107,7 +107,7 @@ module SplinterTreeMachineMod {
   import opened SequenceSetsMod
   import opened ValueMessage
   import opened KeyType
-  import opened InterpMod
+  import opened StampedMapMod
   import opened DiskTypesMod
   import opened AllocationMod
   import opened MsgHistoryMod
